examples/AKE/AKE_proof.ec
@@ -9,8 +9,13 @@ require import Real.
 require import AKE_defs.
 require import AKE_g0.
 
+pred test_fresh(t : Sid option, evs : Event list) =
+  t <> None /\ fresh (proj t) evs.
+
+(* For some small eps to be determined later, we want to prove *)
 const eps : real.
 
-lemma Correct:
+lemma Secure:
   forall (A <: Adv) &m,
-    2%r * Pr[ AKE(A).main() @ &m : res /\ AKE.test <> None /\ (fresh (proj AKE.test) AKE.evs) ] - 1%r < eps.
+    2%r * Pr[   AKE(A).main() @ &m : res /\ test_fresh AKE.test AKE.evs] - 1%r < eps
+by admit.
